Escallon/LR_Parsing/Shift_Reduce_PDA.thy
@@ -6,13 +6,13 @@ begin
 
 datatype ('n, 't) srpda_state = Sym "('n, 't) sym" | Init | Final
 
-fun destSym :: "('n, 't) srpda_state  \<Rightarrow> ('n, 't) sym" where 
-\<open>destSym (Sym X) = X\<close>
+lemma map_Sym_inject_iff[simp]: "map Sym xs = map Sym ys \<longleftrightarrow> xs = ys" 
+  by (metis list.inj_map_strong srpda_state.inject)
 
 definition SRPDA :: "('n, 't) Cfg \<Rightarrow> (('n, 't) srpda_state, 't) gpda" where
   "SRPDA G \<equiv> \<lparr>gpda.states = UNIV, init = Init, final = {Final}, 
-    nxt = {([q], x, [Sym (Tm x), q])|x q. q \<in> UNIV \<and> x \<in> UNIV}, 
-    eps = {(\<alpha>, [Sym (Nt A)])|A \<alpha>. (A, map destSym \<alpha>) \<in> Prods G} 
+    nxt = range (\<lambda>(q, x). ([q], x, [Sym (Tm x), q])), 
+    eps = {(map Sym (rev \<alpha>), [Sym (Nt A)])|A \<alpha>. (A, \<alpha>) \<in> Prods G} 
         \<union> {([Sym (Nt (Start G)), Init], [Final])}\<rparr>"
 
 locale srpda = Extended_Cfg G for G :: "('n::fresh0, 't) Cfg" +
@@ -20,12 +20,46 @@ locale srpda = Extended_Cfg G for G :: "('n::fresh0, 't) Cfg" +
   assumes srpda: "M = SRPDA G"
 begin
 
+lemma srpda_init [simp]:
+  "gpda.init M = Init" using srpda unfolding SRPDA_def by simp
+
+lemma srpda_nxt [simp]:
+  "gpda.nxt M = range (\<lambda>(q, x). ([q], x, [Sym (Tm x), q]))" 
+  using srpda unfolding SRPDA_def by simp
+
+lemma srpda_eps [simp]:
+  "gpda.eps M = {(map Sym (rev \<alpha>), [Sym (Nt A)])|A \<alpha>. (A, \<alpha>) \<in> Prods G} 
+    \<union> {([Sym (Nt (Start G)), Init], [Final])}"
+  using srpda unfolding SRPDA_def by simp
+
 type_synonym ('nts, 'tms) config = "('nts, 'tms) srpda_state list \<times> 'tms list"
 
 inductive step :: "('n, 't) config \<Rightarrow> ('n, 't) config \<Rightarrow> bool" 
   (infix \<open>\<turnstile>\<close> 55) where
-step_nxt[intro]: "(ps, a, qs) \<in> nxt M \<Longrightarrow> (ps@rs, a#w) \<turnstile> (qs@rs, w)" |
-step_eps[intro]: "(ps, qs) \<in> eps M \<Longrightarrow> (ps@rs, w) \<turnstile> (qs@rs, w)"
+step_nxt[intro]: "(xs, a, ys) \<in> nxt M \<Longrightarrow> (xs@zs, a#w) \<turnstile> (ys@zs, w)" |
+step_eps[intro]: "(xs, ys) \<in> eps M \<Longrightarrow> (xs@zs, w) \<turnstile> (ys@zs, w)"
+
+lemma step_cases [consumes 1, case_names shift reduce finish, cases set: srpda.step]:
+  assumes "c0 \<turnstile> c1"
+  obtains 
+    x xs a w where "c0 = (x # xs, a # w)" "c1 = (Sym (Tm a) # x # xs, w)" |
+    A \<alpha> xs w where "(A, \<alpha>) \<in> Prods G" "c0 = (map Sym (rev \<alpha>) @ xs, w)" "c1 = (Sym (Nt A) # xs, w)" |
+        xs w where "c0 = (Sym (Nt (Start G)) # Init # xs, w)" "c1 = (Final # xs, w)"
+  using assms by cases auto
+
+lemma shifts [simp]:
+  "(x # xs, a # w) \<turnstile> (Sym (Tm a) # x # xs, w)"
+  using step_nxt by fastforce
+
+lemma reduces [simp]:
+  assumes "(A, \<alpha>) \<in> Prods G"
+  shows "(map Sym (rev \<alpha>) @ \<beta>, w) \<turnstile> (Sym (Nt A) # \<beta>, w)"
+  using assms step_eps by (metis (mono_tags, lifting) Un_insert_right append.simps(1,2) 
+      insert_iff mem_Collect_eq srpda_eps sup_bot.right_neutral)
+
+lemma finishes [simp]:
+  "(Sym (Nt (Start G)) # Init # \<alpha>, w) \<turnstile> (Final # \<alpha>, w)"
+  using step_eps by fastforce
 
 abbreviation steps :: "('n, 't) config \<Rightarrow> ('n, 't) config \<Rightarrow> bool" (infix \<open>\<turnstile>*\<close> 55) where
   "steps \<equiv> step\<^sup>*\<^sup>*"
@@ -33,16 +67,163 @@ abbreviation steps :: "('n, 't) config \<Rightarrow> ('n, 't) config \<Rightarro
 abbreviation stepn :: "('n, 't) config \<Rightarrow> nat \<Rightarrow> ('n, 't) config \<Rightarrow> bool" (\<open>_ \<turnstile>'(_') _\<close> 55) where
   "c\<^sub>0 \<turnstile>(n) c\<^sub>1 \<equiv> (step ^^ n) c\<^sub>0 c\<^sub>1"
 
+lemma reachable_imp_substring:
+  assumes "(xs, w) \<turnstile>* (ys, v)"
+  obtains u where "w = u @ v"
+  using assms proof (induction "(ys, v)" arbitrary: ys v thesis rule: rtranclp_induct)
+  case (step y)
+  from step(2) show ?case proof (cases rule: step.cases)
+    case (step_nxt rs a ss ts)
+    with step(3)[of _ "a # v"] step(4)[of "_ @ [a]"] show ?thesis by auto
+  qed (use step in auto)
+qed simp
+
+lemma steps_len_dec:
+  "(xs, w) \<turnstile>* (ys, v) \<Longrightarrow> length w \<ge> length v"
+  using reachable_imp_substring by fastforce
+
+
+lemma into_Init_impossible:
+  assumes "c \<turnstile> (Init # xs, w)" 
+  shows "False"
+using assms by cases simp_all
+
+lemma Init_not_Suc_reachable:
+  assumes "c\<^sub>0 \<turnstile>(Suc n) (y # ys, v)"
+  shows "y \<noteq> Init"
+  using into_Init_impossible assms by auto
+
+lemma reaches_Init_imp_refl:
+  "c \<turnstile>* (Init # xs, w) \<Longrightarrow> c = (Init # xs, w)"
+  using Init_not_Suc_reachable stepcnt_cases by metis
+
 definition Lang :: "'t list set" where
-  "Lang \<equiv> {w. ([init M], w) \<turnstile>* ([Final], [])}"
+  "Lang \<equiv> {w. ([Init], w) \<turnstile>* ([Final], [])}"
 
 lemma in_Lang_imp_reaches_S:
-  "w \<in> Lang \<Longrightarrow> ([init M], w) \<turnstile>* ([Sym (Nt (Start G)), Init], [])"
-  sorry
+  assumes "w \<in> Lang" 
+  shows "([Init], w) \<turnstile>* ([Sym (Nt (Start G)), Init], [])"
+proof -
+  from assms have "([Init], w) \<turnstile>* ([Final], [])" unfolding Lang_def by simp
+  thus ?thesis proof cases
+    case (rtrancl_into_rtrancl c)
+    from this(2) show ?thesis 
+      by cases (use rtrancl_into_rtrancl(1) in blast)+
+  qed
+qed
+
+lemma prefix_consumable:
+  "(X # \<alpha>, u @ v) \<turnstile>* (map (Sym \<circ> Tm) (rev u) @ X # \<alpha>, v)"
+proof (induction u arbitrary: X \<alpha>)
+  case (Cons a u)
+  have "(X # \<alpha>, (a # u) @ v) \<turnstile> (Sym (Tm a) # X # \<alpha>, u @ v)"
+    by simp
+  also from Cons.IH have "... \<turnstile>* (map (Sym \<circ> Tm) (rev u) @ (Sym \<circ> Tm) a # X # \<alpha>, v)"
+    by fastforce
+  finally show ?case 
+    by (metis (no_types, lifting) append.assoc append_Cons append_Nil list.simps(9) rev.simps(2)
+        rev_map)
+qed auto
+
+lemma Tm_top_of_stack_imp_consumed:
+  assumes "c \<turnstile> (Sym (Tm a) # \<alpha>, w)" 
+  shows "c = (\<alpha>, a # w)"
+  using assms by cases auto
+
+lemma eps_step_stack_indep:
+  assumes "(\<alpha>, u) \<turnstile> (\<beta>, u)"
+  shows "(\<alpha>, v) \<turnstile> (\<beta>, v)"
+  using assms by cases 
+    (simp, 
+      (smt (verit, ccfv_threshold) assms not_Cons_self2 prod.inject srpda.step.cases 
+        srpda.step_eps srpda_axioms)+)
+
+lemma eps_stack_indep:
+  "(\<alpha>, u) \<turnstile>* (\<beta>, u) \<Longrightarrow> (\<alpha>, v) \<turnstile>* (\<beta>, v)"
+proof (induction "(\<alpha>, u)" arbitrary: \<alpha> rule: converse_rtranclp_induct)
+  case (step c)
+  then obtain \<gamma> w where "c = (\<gamma>, w)" using old.prod.exhaust by metis
+  with step(1) have c_\<gamma>u: "c = (\<gamma>, u)"
+    using steps_len_dec step.cases step.hyps(2) by fastforce
+  with step(1) eps_step_stack_indep have "(\<alpha>, v) \<turnstile> (\<gamma>, v)" by blast
+  with step(3) c_\<gamma>u show ?case by simp
+qed simp
+
+lemma tl_indep:
+  "(\<alpha>, u @ v) \<turnstile>* (\<gamma>, v) \<Longrightarrow> (\<alpha>, u @ w) \<turnstile>* (\<gamma>, w)"
+proof (induction "(\<alpha>, u @ v)" arbitrary: \<alpha> u rule: converse_rtranclp_induct)
+  case (step c)
+  show ?case proof (cases u)
+    case Nil
+    then show ?thesis using step(1,2) eps_stack_indep 
+      by (metis append_Nil converse_rtranclp_into_rtranclp)
+  next
+    case (Cons a u')
+    from step(1) show ?thesis 
+      using step Cons by cases 
+        (metis (no_types, lifting) append_Cons list.inject shifts converse_rtranclp_into_rtranclp 
+          prod.inject,
+         metis (no_types, lifting) reduces converse_rtranclp_into_rtranclp prod.inject,
+         metis (no_types, lifting) finishes converse_rtranclp_into_rtranclp prod.inject)
+  qed
+qed simp
+
+lemma Tms_on_stack_imp_consumed:
+  "(\<alpha>, u @ v @ w) \<turnstile>* (map (Sym \<circ> Tm) (rev v) @ \<beta>, w) \<Longrightarrow> (\<alpha>, u @ v @ w) \<turnstile>* (\<beta>, v @ w)"
+proof (induction v arbitrary: u w rule: rev_induct)
+  case (snoc a v)
+  from this(2) have 
+    "(\<alpha>, u @ (v @ [a]) @ w) \<turnstile>* (map (Sym \<circ> Tm) (rev v) @ \<beta>, a # w)" (is "?steps")
+    "(map (Sym \<circ> Tm) (rev v) @ \<beta>, a # w) \<turnstile> (map (Sym \<circ> Tm) (rev (v @ [a])) @ \<beta>, w)" (is "?step")
+  proof -
+    from snoc(2) have "?steps \<and> ?step" proof cases
+      case (rtrancl_into_rtrancl c)
+      then show ?thesis using Tm_top_of_stack_imp_consumed by simp
+    qed simp
+    thus ?steps ?step by auto
+  qed
+  with snoc.IH show ?case by fastforce
+qed simp
+
+lemma invariant:
+  "Prods G \<turnstile> \<alpha> \<Rightarrow>r* map Tm w \<Longrightarrow> ([Init], w) \<turnstile>* (map Sym (rev \<alpha>) @ [Init], [])"
+proof (induction \<alpha> rule: converse_rtranclp_induct)
+  case base
+  then show ?case using prefix_consumable[of _ _ w "[]"] 
+    by (simp add: rev_map)
+next
+  case (step \<alpha> \<beta>)
+  from step(1) show ?case proof cases
+    case (1 A \<delta> \<gamma> v)
+    from this(2) step(2) obtain u where "w = u @ v" 
+      using derives_append_map_Tm[of _ "\<gamma> @ \<delta>" "map Tm v"] derivers_iff_derives 
+      by (metis append.assoc derives_map_Tm_iff map_Tm_inject_iff)
+    with 1 Tms_on_stack_imp_consumed[of _ _ _ "[]"] step 
+      have "([Init], w) \<turnstile>* (map Sym (rev (\<gamma> @ \<delta>)) @ [Init], v)"
+      by (simp add: rev_map)
+    also have "... \<turnstile> (Sym (Nt A) # map Sym (rev \<gamma>) @ [Init], v)"
+      using 1(3) by simp
+    also have "... \<turnstile>* (map (Sym \<circ> Tm) (rev v) @ Sym (Nt A) # map Sym (rev \<gamma>) @ [Init], [])"
+      using prefix_consumable[of _ _ v "[]"] by simp
+    finally show ?thesis
+      using 1(1) by (simp add: rev_map)
+  qed
+qed
 
 lemma srpda_complete:
   "LangS G \<subseteq> Lang"
-  sorry
+proof
+  fix w
+  assume "w \<in> LangS G"
+  hence "Prods G \<turnstile> [Nt (Start G)] \<Rightarrow>r* map Tm w"
+    unfolding Context_Free_Grammar.Lang_def using derivers_iff_derives by fast
+  with invariant have "([Init], w) \<turnstile>* ([Sym (Nt (Start G)), Init], [])"
+    by fastforce
+  also have "... \<turnstile> ([Final], [])"
+    using step_eps by fastforce
+  finally show "w \<in> Lang"
+    unfolding Lang_def by blast
+qed
 
 end
 end
